WIP

common/Events.v
@@ -2120,3 +2120,73 @@ Section INFORM_TRACES_PRESERVED.
   Qed.
 
 End INFORM_TRACES_PRESERVED.
+
+
+Section LEAK.
+
+  Definition block_first_order (m: mem) (b: block): Prop :=
+    forall (ofs: Z),
+      match (ZMap.get ofs (Mem.mem_contents m) !! b) with
+      | Fragment vv _ _ => not_ptr vv
+      | _ => True
+      end.
+
+  (* Public symbols are visible outside the compilation unit, 
+     so when interacting via external calls, limit them to first-order. *)
+  Definition public_first_order (ge: Senv.t) (m: mem) :=
+    forall id b (PUBLIC: Senv.public_symbol ge id = true) (FIND: Senv.find_symbol ge id = Some b),
+      block_first_order m b.
+
+  Definition val_first_order (m: mem) (v: val): Prop :=
+    match v with
+    | Vptr b _ => block_first_order m b
+    | Vundef => False
+    | _ => True
+    end.
+
+  Definition vals_first_order (m: mem) (vs: list val): Prop :=
+    Forall (val_first_order m) vs.
+
+  Definition block_public (ge: Senv.t) (b: block): Prop :=
+    exists id, Senv.invert_symbol ge b = Some id /\ Senv.public_symbol ge id = true.
+
+  Definition val_public (ge: Senv.t) (v: val): Prop :=
+    match v with
+    | Vptr b _ => block_public ge b
+    | Vundef => False
+    | _ => True
+    end.
+
+  Definition vals_public (ge: Senv.t) (vs: list val): Prop :=
+    Forall (val_public ge) vs.
+
+  Definition limit_leaks (ge: Senv.t) (m: mem) (args: list val): Prop :=
+    public_first_order ge m /\ vals_public ge args.
+
+  Lemma limit_leaks_ensures_args_first_order
+        ge m args
+        (LL: limit_leaks ge m args)
+    :
+    vals_first_order m args.
+  Proof.
+    revert LL. induction args; intros; simpl. econstructor.
+    inv LL. inv H0. econstructor; eauto.
+    - destruct a; simpl in *; auto. destruct H3 as (id & INV & PUB).
+      apply Senv.invert_find_symbol in INV. specialize (H id b PUB INV). auto.
+    - apply IHargs. red. auto.
+  Qed.
+
+  Definition limit_leaks_if_unknown
+             (ef: external_function) (ge: Senv.t) (m: mem) (args: list val) : Prop :=
+    match ef with
+    | EF_external name cp sg => limit_leaks ge m args
+    | EF_builtin name sg | EF_runtime name sg =>
+                             match lookup_builtin_function name sg with
+                             | None => limit_leaks ge m args
+                             | _ => True
+                             end
+    | EF_inline_asm txt sg clb => limit_leaks ge m args
+    | _ => True
+    end.
+
+End LEAK.
